Add examples

denotational/System.v
@@ -20,6 +20,8 @@ From ExtLib Require Import
      String
      Monad.
 
+From DSL Require Import Vectors.
+
 Import ITreeNotations.
 Import MonadNotation.
 Local Open Scope monad_scope.
@@ -32,29 +34,47 @@ Notation fin := t.
 
 (** Some general Sets needed for Systems work *)
 Module Type Systems.
-  Parameter uid: Set.             (** Principal *)
+
+  Parameter uid: nat -> Set.      (** Principal *)
   Parameter bytestring: Set.      (** ByteString *)
   Parameter var : Set.            (** binders *)
   Parameter channel: Type -> Set. (** Typed channels *)
-  Parameter eqdec_uid: RelDec (@eq uid).
+  
   Parameter eqdec_bytestring: RelDec (@eq bytestring).
   Parameter eqdec_var: RelDec (@eq var).
   Parameter eqdec_channel: forall T, RelDec (@eq (channel T)).
-
-  Global Existing Instance eqdec_uid.
+  Parameter eqdec_uid: forall t, RelDec (@eq (uid t)).
+  
   Global Existing Instance eqdec_bytestring.
   Global Existing Instance eqdec_var.
   Global Existing Instance eqdec_channel.
-  
+  Global Existing Instance eqdec_uid.
+
+  Parameter uid_coerce: forall t, uid t -> fin t.
+  Global Coercion uid_coerce: uid >-> fin.
+  Parameter fin_coerce: forall t, fin t -> uid t.
+  Global Coercion fin_coerce: fin >-> uid.
 End Systems.
 
-(** Specialize var to strings and channels to nat *)
-Module Type SSystem <: Systems.
-  Parameter uid: Set.                 (** Principal *)
-  Parameter bytestring: Set.          (** ByteString *)
+Module DistrSystem <: Systems.
   
-  Parameter eqdec_uid: RelDec (@eq uid).
-  Parameter eqdec_bytestring: RelDec (@eq bytestring).
+  Definition uid := fin.
+
+  Definition uid_coerce t (a: uid t) := id a.
+  Definition fin_coerce t (a: fin t) := id a.
+  
+  Equations reldec_uid: forall t, fin t -> fin t -> bool :=
+    reldec_uid F1 F1 := true;
+    reldec_uid (FS i) (FS j) := reldec_uid i j;
+    reldec_uid _ _ := false.
+  
+  (** Decidable UIDs *)
+  Global Instance eqdec_uid: forall t, RelDec (@eq (uid t)) := {
+      rel_dec a b := @reldec_uid t a b
+    }.
+  
+  Definition bytestring := nat.  
+  Global Instance eqdec_bytestring: RelDec (@eq bytestring) := _.
   
   Definition var : Set := string.     (** binders *)
   Definition channel(T: Type) := nat. (** Typed channels *)
@@ -62,36 +82,20 @@ Module Type SSystem <: Systems.
   Definition eqdec_var: RelDec (@eq var) := _.
   Definition eqdec_channel: forall T, RelDec (@eq (channel T)) :=
     fun T => _.
+ 
+End DistrSystem.
 
-End SSystem.
-
-Module Net(S: Systems).
+Module Messaging(S: Systems).
   Import S.
 
-  (** Number of agents *)
-  Parameter n: nat.
-
-  (** UID is a fin. This is enforced by the type signature of `choice` in CTrees *)
-  Definition uid := fin n.
-
-  Equations reldec_uid: forall t, fin t -> fin t -> bool :=
-    reldec_uid F1 F1 := true;
-    reldec_uid (FS i) (FS j) := reldec_uid i j;
-    reldec_uid _ _ := false.
-  
-  (** Decidable UIDs *)
-  Global Instance eqdec_uid: RelDec (@eq uid) := {
-      rel_dec a b := @reldec_uid n a b
-    }.
-
-  (** Messages exchagend *)
-  Record Msg := {
-      principal: uid;
+   (** Messages exchagend *)
+  Record Msg t := {
+      principal: uid t;
       payload: bytestring
     }.
 
   (** Decidable messages *)
-  Global Instance eqdec_msg: RelDec (@eq Msg) := {
+  Global Instance eqdec_msg: forall t, RelDec (@eq (Msg t)) := {
       rel_dec m1 m2 := match m1, m2 with
                          {| principal := u1; payload := p1 |},
                          {| principal := u2; payload := p2 |} =>
@@ -100,49 +104,52 @@ Module Net(S: Systems).
     }.
 
   (** A queue of messages received *)
-  Definition queue := list Msg.
+  Definition queue t := list (Msg t).
 
   (** A task is either running or returned *)
-  Inductive Task(E: Type -> Type)(T: Type) :=
-  | Done (r: T)(q: queue)
-  | Running (c: itree E T)(q: queue).
+  Inductive Task t (E: Type -> Type)(T: Type) :=
+  | Done (r: T)(q: queue t)
+  | Running (c: itree E T)(q: queue t).
 
-  Definition is_done{E T}(t: Task E T) :=
+  Definition is_done{E T n}(t: Task n E T) :=
     match t with
     | Done _ _ => true
     | Running _ _ => false
     end.
 
-  Definition is_running{E T}(t: Task E T) :=
+  Definition is_running{E T n}(t: Task n E T) :=
     match t with
     | Done _ _ => false
     | Running _ _ => true
     end.
-
+  
   (** Network effects *)
-  Inductive Net: Type -> Type :=
-  | Recv: Net Msg 
-  | Send : Msg -> Net unit
+  Inductive Net{n: nat}: Type -> Type :=
+  | Recv: Net (Msg n)
+  | Send : (Msg n) -> Net unit
   | Broadcast: bytestring -> Net unit.
 
-  Definition recv {E} `{Net -< E}: itree E Msg := embed Recv.
-  Definition send {E} `{Net -< E}: Msg -> itree E unit := embed Send.
-  Definition broadcast {E} `{Net -< E}: bytestring -> itree E unit := embed Broadcast.
-End Net.
+  Definition recv {E n} `{Net -< E}: itree E (Msg n) := embed Recv.
+  Definition send {E n} `{Net -< E}: Msg n -> itree E unit := embed Send.
+  Definition broadcast {E n} `{Net -< E}: bytestring -> itree E unit :=
+    embed (@Broadcast n).
 
+End Messaging.
 
 Module PKI(S: Systems).
   Import S.
-  Definition Enc (p: uid) := bytestring.
-  Definition Sig (p: uid) := bytestring.
-  Definition Pub (p: uid) := bytestring.
-  Definition Priv (p: uid) := bytestring.
+  Context {n: nat}.
+
+  Definition Enc (p: uid n) := bytestring.
+  Definition Sig (p: uid n) := bytestring.
+  Definition Pub (p: uid n) := bytestring.
+  Definition Priv (p: uid n) := bytestring.
   
   Inductive PKI: Type -> Type :=
-  | EncPub(p: uid)(k: Pub p)(plain: bytestring): PKI (Enc p)
-  | DecPriv(p: uid)(k: Priv p)(cipher: Enc p): PKI bytestring
-  | SignPriv(p: uid)(k: Priv p)(plain: bytestring): PKI (Sig p)
-  | CheckPub(p: uid)(k: Pub p)(signed: Sig p): PKI bool.
+  | EncPub(p: uid n)(k: Pub p)(plain: bytestring): PKI (Enc p)
+  | DecPriv(p: uid n)(k: Priv p)(cipher: Enc p): PKI bytestring
+  | SignPriv(p: uid n)(k: Priv p)(plain: bytestring): PKI (Sig p)
+  | CheckPub(p: uid n)(k: Pub p)(signed: Sig p): PKI bool.
 
   Definition encrypt {E} `{PKI -< E} := embed EncPub.
   Definition decrypt {E} `{PKI -< E} := embed DecPriv.
@@ -168,20 +175,25 @@ Module Spawn(S: Systems).
     ITree.trigger (@Block F t c).
 End Spawn.  
 
-
 Module Storage(S: Systems).
-  Import S.
+  Import S Monads.
 
-  Notation heap := (alist var bytestring) (only parsing).
   Definition Map_heap := Map_alist eqdec_var bytestring.
-  Local Existing Instance Map_heap.
-
-  Notation Storage := (stateE heap) (only parsing).
+  Global Existing Instance Map_heap.
   
-  Definition load {E} `{stateE heap -< E}(v: var): itree E (option bytestring) :=
+  Notation heap := (alist var bytestring).
+  Notation Storage := (stateE heap).
+  
+  Definition load {E} `{Storage -< E}(v: var): itree E (option bytestring) :=
     get >>= fun s => ret (lookup v s).
 
-  Definition store {E} `{stateE heap -< E}(v: var)(b: bytestring): itree E unit :=
+  Definition store {E} `{Storage -< E}(v: var)(b: bytestring): itree E unit :=
     get >>= fun s => put (add v b s).
+
+    (** Evaluates, takes a single heap for all agents *)
+  Definition run_storage{E R m}(a: vec m (itree (Storage +' E) R)):
+    stateT heap (fun T => vec m (itree E T)) R :=
+    fun st => Vector.map (fun it => run_state it st) a.
+
 End Storage.  
 
