denotational/Examples.v
@@ -1,0 +1,73 @@
+From ITree Require Import
+     ITree
+     Events.State
+     Events.StateFacts.
+
+From Coq Require Import
+     Fin
+     String.
+
+From ExtLib Require Import
+     RelDec
+     Functor
+     Traversable
+     Monads
+     Option.
+
+From CTree Require CTrees.
+
+From DSL Require Import
+     System
+     Network
+     Vectors.
+
+Import ITreeNotations.
+
+Local Open Scope itree_scope.
+Local Open Scope string_scope.
+Local Open Scope vector_scope.
+
+Set Implicit Arguments.
+Set Contextual Implicit.
+
+(** Utility use the standard library *)
+Definition default{T}(o: option T)(d: T): T :=
+  match o with
+  | None => d
+  | Some v => v
+  end.
+
+Module Examples.
+  Module Network := Network(DistrSystem).                               
+  Import Network DistrSystem.
+
+  (** Some uids *)
+  Program Definition alice : uid 2 := @of_nat_lt 0 2 _.
+  Program Definition bob : uid 2 := @of_nat_lt 1 2 _.
+
+  (** Some programs *)
+  Definition example_alice :=
+    a <- load "a";;
+    send {| principal := bob; payload := default a 0 |};;
+    a' <- recv;;
+    store "b" (payload a').
+
+  Definition example_bob: itree (Storage +' @Net 2) unit :=
+    m <- recv ;;
+    send {| principal := principal m; payload := S (payload m) |}.
+
+  (** A Single agent program *)
+  Definition example: itree (Storage +' @Net 1) unit :=
+    a <- load "a";;
+    store "b" (S (default a 0)).
+
+  Definition S1 := [example].
+  Definition S2 := [example_alice; example_bob].
+
+  Definition C1 := run_network (run_storage S1) List.nil.
+  Definition C2 := run_network (run_storage S2) List.nil.
+
+  Check C1.
+  Check C2.
+End Examples.
+    
