denotational/Network.v
@@ -10,7 +10,6 @@ From CTree Require Import
 
 From ExtLib Require Import
      Monad
-     List
      Traversable
      RelDec.
 
@@ -19,7 +18,7 @@ From Coq Require Import
      Fin (* fin definition here *)
      Program.Equality
      Lia.
-From Coq Require List.
+
 From Equations Require Import
      Equations.
 
@@ -28,36 +27,35 @@ From DSL Require Import
      Vectors.
 
 Import CTrees.CTreeNotations.
-Import VectorNotations.
-Import VectorUtils.
+
 Local Open Scope ctree_scope.
 Local Open Scope vector_scope.
 Local Open Scope fin_vector_scope.
 
-(** Network *)
-Module Network(S: SSystem).
-  Module Net := Net(S).
-  Module Storage := Storage(S).
-  Export Net Storage S.
-  
-  (** Local storage and message passing effects *)
-  Notation Sys := (Storage +' Net) (only parsing).
+Set Implicit Arguments.
+Set Contextual Implicit.
 
-  Fixpoint num_done{E A m}(a: vec m (Task E A)): nat :=
+(** Network *)
+Module Network(S: Systems).
+  Module Messaging := Messaging(S).
+  Module Storage := Storage(S).
+  Export Monads Storage Messaging S.
+
+  Fixpoint num_done{E A m n}(a: vec m (Task n E A)): nat :=
     match a with
     | ((Done _ _) :: ts) => S (num_done ts)
     | ((Running _ _) :: ts) => num_done ts
     | [] => 0
     end.
 
-  Fixpoint num_running{E A m}(a: vec m (Task E A)): nat :=
+  Fixpoint num_running{E A m n}(a: vec m (Task n E A)): nat :=
     match a with
     | ((Done _ _) :: ts) => num_running ts
     | ((Running _ _) :: ts) => S (num_running ts)
     | [] => 0
     end.
 
-  Lemma done_running_inv: forall A E m (v: vec m (Task E A)),
+  Lemma done_running_inv: forall A E m n (v: vec m (Task n E A)),
       num_done v + num_running v = m.
   Proof.
     intros.
@@ -70,20 +68,19 @@ Module Network(S: SSystem).
           rewrite IHv; reflexivity.
   Defined.
 
-
-  Equations absolute_idx{E A m}(v: vec m (Task E A))(i: fin (num_running v)): (fin m * itree E A * queue) :=
-    absolute_idx ((Running _ _) :: ts) (FS k) :=
-      match absolute_idx ts k with
-      | (i, a, q) => (FS i, a, q)
-      end;
-    absolute_idx ((Done a b) :: ts) k :=
-      match absolute_idx ts k with
-      | (i, a, q) => (FS i, a, q)
-      end;
-    absolute_idx ((Running a q) :: ts) F1 := (F1, a ,q).
-
-  Definition schedule_network_0{E A m}(a: vec m (Task E A))
-             {H: num_running a = 0}: vec m (A * queue).
+  Equations get_running{E A m n}(v: vec m (Task n E A))
+            (i: fin (num_running v)): (fin m * itree E A * queue n) :=
+    get_running ((Running _ _) :: ts) (FS k) := match get_running ts k with
+                                                 | (i, a, q) => (FS i, a, q)
+                                                 end;
+    get_running ((Done a b) :: ts) k := match get_running ts k with
+                                         | (i, a, q) => (FS i, a, q)
+                                         end;
+    get_running ((Running a q) :: ts) F1 := (F1, a ,q).
+  Transparent get_running.
+  
+  Definition schedule_network_0{E A m n}(a: vec m (Task n E A))
+             {H: num_running a = 0}: vec m (A * queue n).
     dependent induction a.
     - exact [].
     - destruct h; cbn in *.
@@ -91,54 +88,55 @@ Module Network(S: SSystem).
       + inversion H.
   Defined.
 
-  (** Messaging scheduler (Send, Receive, Broadcast *)
-  Equations schedule_network_Sn {R: Type}
-            (schedule: vec n (Task Net R) ->
-                       CTrees.ctree void1 (vec n (R * queue)))
-            (sys: vec n (Task Net R))
-            {H: exists m, num_running sys = S m}:
-    CTrees.ctree void1 (vec n (R * queue)) :=
-    schedule_network_Sn schedule sys :=
-      (** Non-det pick an agent that is running to execute *)
-      r <- choice true (num_running sys) ;;
-      (** q: the message queue of i *)
-      let (p, q) := absolute_idx sys r in
-      (** i: The absolute index of a running agent `r`
-              a: The itree of agent `i` (Running) *)
-      let (i, a) := p in
-      (** Observe the itree `a` *)
-      match observe a with
-      | RetF v =>
-          CTrees.TauI (schedule (sys @ i := Done v q))
-      | TauF t =>
-          CTrees.TauI (schedule (sys @ i := Running t q))
-      | VisF (Send msg) k =>
-          let sys' := sys @ i := Running (k tt) q in
-          let recp := principal msg in
-          match sys $ recp with
-          | Running a q =>
-              let msg' := {| principal := i; payload := payload msg |} in
-              CTrees.TauV (schedule (sys' @ recp := Running a (List.cons msg' q)))
-          | Done _ _ => CTrees.TauV (schedule sys')
-          end
-      (** TODO: Msg delivery non-determinism *)
-      | VisF Recv k =>
-          match last q with 
-          | Some msg =>
-              (** Pop the msg from the end *)
-              CTrees.TauV (schedule (sys @ i := Running (k msg) (init q)))
-          | None =>
-              (** Just loop again if no messages in q *)
-              CTrees.TauI (schedule sys)
-          end
-      | VisF (Broadcast b) k =>
-          let msg := {| principal := i; payload := b |} in
-          let sys' := sys @ i := Running (k tt) q in
-          CTrees.TauV (schedule (map (fun a =>
-                                        match a with
-                                        | Running a q => Running a (List.cons msg q)
-                                        | Done a q => Done a q
-                                        end) sys'))
+  Equations schedule_network{R: Type}{n: nat}
+             (schedule: vec n (Task n (@Net n) R) ->
+                        CTrees.ctree void1 (vec n (R * queue n)))
+             (sys: vec n (Task n (@Net n) R)):
+    CTrees.ctree void1 (vec n (R * queue n)) :=
+    schedule_network schedule sys :=
+      match num_running sys as n1 return (num_running sys = n1 -> CTrees.ctree void1 (vec n (R * queue n))) with
+      | 0 => fun Hnr: num_running sys = 0 => CTrees.Ret (schedule_network_0 sys)
+      | S n1 =>
+          fun Hnr: num_running sys = S n1 => 
+            (** Non-det pick an agent that is running to execute *)
+            r <- choice true (num_running sys) ;;
+            (** q: the message queue of i *)
+            let (p, q) := get_running sys r in
+            (** i: The absolute index of a running agent `r`
+                a: The itree of agent `i` (Running)        *)    
+            let (i, a) := p in
+            (** Observe the itree `a` *)
+            match observe a with
+            | RetF v =>
+                CTrees.TauI (schedule (sys @ i := Done v q))
+            | TauF t =>
+                CTrees.TauI (schedule (sys @ i := Running t q))
+            | VisF (Send msg) k =>
+                let sys' := sys @ i := Running (k tt) q in
+                let recp := principal msg in
+                match sys' $ recp with
+                | Running a q =>
+                    let msg' := {| principal := i; payload := payload msg |} in
+                    CTrees.TauV (schedule (sys' @ recp := Running a (List.cons msg' q)))
+                | Done _ _ => CTrees.TauV (schedule sys')
+                end
+            (** TODO: Msg delivery non-determinism *)
+            | VisF Recv k =>
+                match last q with 
+                | Some msg =>
+                    (** Pop the msg from the end *)
+                    CTrees.TauV (schedule (sys @ i := Running (k msg) (init q)))
+                | None =>
+                    (** Just loop again if no messages in q *)
+                    CTrees.TauI (schedule sys)
+                end
+            | VisF (Broadcast b) k =>
+                let msg := {| principal := i; payload := b |} in
+                let sys' := map (fun a => match a with
+                                          | Running a q => Running a (List.cons msg q)
+                                          | Done a q => Done a q
+                                          end) sys in 
+                CTrees.TauV (schedule (sys' @ i := Running (k tt) q))
           (** TODO: NON-det version 
             sys'' <- mapT (fun a: list Msg * itree Net R =>
                           let (q', a') := a in
@@ -148,18 +146,19 @@ Module Network(S: SSystem).
             
             CTrees.TauV (schedule sys'' done)
           *)
-      end.
+            end
+      end eq_refl.
+      
+  CoFixpoint schedule {R: Type}{n: nat} := @schedule_network R n schedule.
 
-  Definition schedule_network{R: Type}
-             (schedule: vec n (Task Net R) ->
-                        CTrees.ctree void1 (vec n (R * queue)))
-             (sys: vec n (Task Net R)): CTrees.ctree void1 (vec n (R * queue)).
-    destruct (num_running sys) eqn:Hnr.
-    - refine (CTrees.Ret (schedule_network_0 sys)); assumption.
-    - refine (schedule_network_Sn schedule sys); exists n0; assumption.
-  Defined.
-
-  CoFixpoint schedule {R: Type} := @schedule_network R schedule.
-
+  
+  (** Evaluates Net *)
+  Definition run_network{R m}(a: stateT heap (fun T => vec m (itree (@Net m) T)) R):
+    stateT heap (fun T => (CTrees.ctree void1 (vec m T))) (R * queue m) :=
+    fun st => (** Need to change the associativity on tuples here, TODO: fix if possible *)
+      CTrees.CTree.map (Vector.map (fun triple => match triple with
+                                                  | (h, r, q) => (h, (r, q))
+                                                  end))
+                       (schedule (Vector.map (fun it =>
+                                                Running it List.nil) (a st))).
 End Network.
-
