denotational/Vectors.v
@@ -5,74 +5,67 @@ From Coq Require Import
 
 From Coq Require List.
 
-Import VectorNotations.
-
 From Equations Require Import Equations.
 
-From DSL Require Import Agent.
+Export VectorNotations.
+Declare Scope fin_vector_scope.
 
-Module VectorUtils.
+Notation vec n T := (Vector.t T n).
+Notation fin := Fin.t.
 
-  Declare Scope fin_vector_scope.
+Equations vector_remove{A n}(v: vec (S n) A)(i: fin (S n)) : vec n A by wf n lt :=
+  vector_remove (h :: h' :: ts) (FS (FS j)) := h :: (vector_remove (h' :: ts) (FS j));
+  vector_remove (h :: h' :: ts) (FS F1) := h :: ts;
+  vector_remove (h :: h' :: ts) F1 := h' :: ts;
+  vector_remove (h::nil) F1 := @nil A.
+Transparent vector_remove.
 
-  Notation vec n T := (Vector.t T n).
-  Notation fin := Fin.t.
+Equations vector_replace{A n}(v: vec n A)(i: fin n)(a: A): vec n A by wf n lt :=
+  vector_replace [] _ _ := [];
+  vector_replace (h :: h' :: ts) (FS (FS j)) a := h :: (vector_replace (h' :: ts) (FS j) a);
+  vector_replace (h :: h' :: ts) (FS F1) a := h :: a :: ts;
+  vector_replace (h :: h' :: ts) F1 a := a :: h' :: ts;
+  vector_replace [h] F1 a := [a].
+Transparent vector_replace.
 
-  Equations vector_remove{A n}(v: vec (S n) A)(i: fin (S n)) : vec n A by wf n lt :=
-    vector_remove (h :: h' :: ts) (FS (FS j)) := h :: (vector_remove (h' :: ts) (FS j));
-    vector_remove (h :: h' :: ts) (FS F1) := h :: ts;
-    vector_remove (h :: h' :: ts) F1 := h' :: ts;
-    vector_remove (h::nil) F1 := @nil A.
-                                                   
-  Equations vector_replace{A n}(v: vec n A)(i: fin n)(a: A): vec n A by wf n lt :=
-    vector_replace [] _ _ := [];
-    vector_replace (h :: h' :: ts) (FS (FS j)) a := h :: (vector_replace (h' :: ts) (FS j) a);
-    vector_replace (h :: h' :: ts) (FS F1) a := h :: a :: ts;
-    vector_replace (h :: h' :: ts) F1 a := a :: h' :: ts;
-    vector_replace [h] F1 a := [a].
+Notation "v '@' i ':=' a" := (vector_replace v i a) (at level 80): fin_vector_scope.
+Notation "v '$' i" := (nth v i) (at level 80): fin_vector_scope.
+Notation "v '--' i" := (vector_remove v i) (at level 80): fin_vector_scope.
 
-  Notation "v '@' i ':=' a" := (vector_replace v i a) (at level 80): fin_vector_scope.
-  Notation "v '$' i" := (nth v i) (at level 80): fin_vector_scope.
-  Notation "v '--' i" := (vector_remove v i) (at level 80): fin_vector_scope.
+(** Vector utils *)
+Equations forallb {A}{m: nat}(f: A -> bool)(a: vec m A): bool :=
+  forallb _ [] := true;
+  forallb f (h :: ts) := andb (f h) (forallb f ts).
+Transparent forallb.
 
-  (** Vector utils *)
-  Equations forallb {A}{m: nat}(f: A -> bool)(a: vec m A): bool :=
-    forallb _ [] := true;
-    forallb f (h :: ts) := andb (f h) (forallb f ts).
-
-  Lemma forall_reflect: forall A (m: nat)(f: A -> bool) (l: vec m A),
-      forallb f l = true <-> Forall (fun x => f x = true) l.
-  Proof.
-    intros A m f l. 
-    split; intros.
-    - dependent induction l.
-      + econstructor.
-      + econstructor; replace (forallb f (h :: l)) with
-            (andb (f h) (forallb f l)) in H by reflexivity;
-          apply andb_prop in H;
-          destruct H.
-        * exact H.
-        * apply IHl; assumption.
-    - dependent induction H.
-      + reflexivity.
-      + replace (forallb f (x :: v)) with
-          (andb (f x) (forallb f v)) by reflexivity.
+Lemma forall_reflect: forall A (m: nat)(f: A -> bool) (l: vec m A),
+    forallb f l = true <-> Forall (fun x => f x = true) l.
+Proof.
+  intros A m f l. 
+  split; intros.
+  - dependent induction l.
+    + econstructor.
+    + econstructor; cbn in H; apply andb_prop in H;
+        destruct H.
+      * exact H.
+      * apply IHl; assumption.
+  - dependent induction H.
+    + reflexivity.
+    + cbn;
         apply andb_true_intro; split; assumption.
-  Defined.
+Defined.
 
-  
-  Fixpoint last{A}(l: list A): option A :=
-    match l with
-    | List.nil => None
-    | List.cons h List.nil => Some h
-    | List.cons h ts => last ts
-    end.
 
-  Fixpoint init{A}(l: list A): list A :=
-    match l with
-    | List.nil => List.nil
-    | List.cons h List.nil => List.nil
-    | List.cons h ts => List.cons h (init ts)
-    end.
-  
-End VectorUtils.
+Fixpoint last{A}(l: list A): option A :=
+  match l with
+  | List.nil => None
+  | List.cons h List.nil => Some h
+  | List.cons h ts => last ts
+  end.
+
+Fixpoint init{A}(l: list A): list A :=
+  match l with
+  | List.nil => List.nil
+  | List.cons h List.nil => List.nil
+  | List.cons h ts => List.cons h (init ts)
+  end.
